Some work on demand functions for selsort
Pardon the messiness!

src/List.v
@@ -299,7 +299,7 @@ Admitted.
 Lemma sum_of_take_cost (n : nat) (xs : list nat) outD
   : outD `is_approx` (lsum (take n xs)) ->
     forall xsA, xsA = Tick.val (sumOfTakeD n xs outD) ->
-    Tick.cost (sumOfTakeD n xs outD) <= 2 * n + 2.
+    Tick.cost (sumOfTakeD n xs outD) <= 2 * n + 3.
 Proof.
   intros. rewrite H. simpl.
   destruct n.
@@ -319,6 +319,76 @@ Proof.
       rewrite length_take_n_leq_n.
       rewrite takeD_cost.
       lia.
+Qed.
+
+(* Select and selsort as given by Software Foundations Chapter 3 *)
+Fixpoint select (x: nat) (l: list nat) : nat * list nat :=
+  match l with
+  | [] => (x, [])
+  | h :: t =>
+    if x <=? h
+    then let (j, l') := select x t in (j, h :: l')
+    else let (j, l') := select h t in (j, x :: l')
+  end.
+
+Fixpoint selection_sort (l : list nat) (n : nat) : list nat :=
+  match l, n with
+  | _, 0 => [] (* ran out of fuel *)
+  | [], _ => []
+  | x :: r, S n' => let (y, r') := select x r in y :: selection_sort r' n'
+end.
+
+(* The entire list must be forced to select smallest element *)
+Definition selectD (x : nat) (xs : list nat) (outD : listA nat) : Tick (T (listA nat)) :=
+  Tick.MkTick (1 + length xs) (exact (x::xs)).
+
+(* The entire list is forced one selection at a time*)
+Fixpoint selection_sortD (xs : list nat) (outD : listA nat) : Tick (T (listA nat)) :=
+  Tick.tick >>
+  match xs, outD with
+  | [], _ => Tick.ret (Thunk NilA)
+  | x :: xs', ConsA zD zsD =>
+    let+ _ := thunkD (selection_sortD xs') zsD in
+    let+ xsD := selectD x xs' NilA in
+    Tick.ret xsD (* We invariably force the entire input list *)
+  | _, _ => bottom
+  end.
+
+Lemma sort_produces_element (n : nat) (x : nat) (xs : list nat) :
+  selection_sort (x :: xs) (S n) = fst (select x xs) :: selection_sort (snd (select x xs)) n.
+Proof.
+  simpl. destruct (select x xs). simpl. reflexivity.
+Qed.
+
+Definition head_def {a} (xs : list a) (d : a) : a :=
+  match xs with
+  | [] => d
+  | x :: _ => x
+  end.
+
+(* We force the empty list or the first element only *)
+Definition headD {a} (xs : list a) (d : a) (outD : a) : Tick (T (listA a)) :=
+  Tick.tick >>
+  match xs with
+  | [] => Tick.ret (Thunk NilA)
+  | x :: _ => Tick.ret (Thunk (ConsA (Thunk x) (Undefined)))
+  end.
+
+Definition head_selection_sortD (xs : list nat) (outD : nat) : Tick (T (listA nat)) :=
+  let+ list_headD := headD (selection_sort xs (length xs)) 0 outD in
+  let+ xsD := thunkD (selection_sortD xs) list_headD in
+  Tick.ret xsD.
+
+Lemma head_selection_sortD_cost (xs : list nat) (outD : nat) :
+  outD `is_approx` head_def (selection_sort xs (length xs)) 0 ->
+  forall xsA, xsA = Tick.val (head_selection_sortD xs outD) ->
+  Tick.cost (head_selection_sortD xs outD) <= length xs + 2.
+Proof.
+  intros. rewrite H. destruct xs.
+  - simpl. lia.
+  - unfold head_selection_sortD.
+    assert (H1 : length (n :: xs) = S (length xs)). auto. rewrite H1.
+    rewrite sort_produces_element. simpl. lia.
 Qed.
 
 (* Fixpoint takeD_ {a : Type} (n : nat) (xs' : list a) (outD : listA a) : Tick (T (listA a) * T (listA a)) :=
